@prefix rdf: <http://www.w3.org/1999/02/22-rdf-syntax-ns#> .
@prefix owl: <http://www.w3.org/2002/07/owl#> .
@prefix rdfs: <http://www.w3.org/2000/01/rdf-schema#> .
@prefix skos: <http://www.w3.org/2004/02/skos/core#> .
@prefix ldp: <http://www.w3.org/ns/ldp#> .
@prefix xsd: <http://www.w3.org/2001/XMLSchema#>.


ldp:Resource a rdfs:Class;
  rdfs:label "ldp Resource";
  rdfs:comment """
     A HTTP resource whose state is represented in any way that conforms to the simple 
     lifecycle patterns and conventions in section 5. Linked Data Platform Resources.
  """ .

ldp:Source a rdfs:Class;
  rdfs:label "ldp Resource";
  rdfs:subClassOf ldp:Resource;
  rdfs:comment """
    an ldp:Resource that is also an rdf source: ie that is an RDF graph.
  """ .

ldp:Container a rdfs:Class, owl:Class;
  rdfs:label "ldp Container";
  rdfs:subClassOf ldp:Source;
  rdfs:comment """
    An LDPR representing a collection of member resources and/or contained documents 
    (RDF Document [rdf11-concepts]  or information resources [WEBARCH]) that responds 
    to client requests for creation, modification, and/or enumeration 
    of its members and documents, and that conforms to the simple lifecycle patterns 
    and conventions in section6. Linked Data Platform Containers.
  """;
  skos:editorialNote """
    As the outermost class of the container hierarchy it may be that the ldp:Container could 
be made to be the same as the ldp:IndirectContainer. But leaving space could allow for further
extensions.    
  """ .

ldp:IndirectContainer a rdfs:Class, owl:Class;
   rdfs:comment """
   A LDPC that has the flexibility of choosing what form its membership triples take, 
   and allows members to be any resources [WEBARCH], defined in the posted document.
   """ .

ldp:DirectContainer a rdfs:Class, owl:Class;
   rdfs:comment """
   A LDPC that has the flexibility of choosing what form its membership triples take, 
   and allows members to be any resources [WEBARCH], not only documents.
   """ .

ldp:BasicContainer a rdfs:Class, owl:Class;
  rdfs:label "BasicContainer";
  rdfs:comment """
  A LDPC that uses a single pre-defined predicate to link to both its contained and 
  member documents (information resources). Posting to an ldp:BasicContainer has
  no extra consequences other than creating an ldp:contains relation from the container to
  the newly created resource.
  """ .
 
ldp:contains a rdf:Property, owl:ObjectProperty;
  rdfs:label "contains";
  rdfs:domain ldp:Container;
  rdfs:range ldp:Resource;
  rdfs:comment """
    the ldp:contains relation relates an ldp:Container to a ldp:Resource ( ie a document of some form )
  """ .

ldp:membershipResource a rdf:Property, owl:FunctionalProperty;
  rdfs:label "membershipResource";
  rdfs:domain ldp:IndirectContainerRule;
  rdfs:range  rdfs:Resource .

rdf:Property a owl:Class .

ldp:hasMemberRelation a rdf:Property, owl:FunctionalProperty, owl:ObjectProperty;
  rdfs:label "hasMemberRelation";
  rdfs:domain ldp:IndirectContainerRule;
  rdfs:range  rdf:Property .
  

ldp:isMemberOfRelation a rdf:Property, owl:FunctionalProperty, owl:ObjectProperty; 
   rdfs:label "isMemberOfRelation";
   owl:subPropertyOf [ owl:propertyChainAxiom ( ldp:hasMemberRelation owl:inverseOf ) ];
   skos:editorialNote """
      the ldp:isMemberOfRelation is the equivalent to the hasMemberRelation followed by the owl:inverseOf property 
   """;
   rdfs:domain ldp:IndirectContainerRule; 
   rdfs:range rdf:Property .

ldp:insertedContentRelation a owl:FunctionalProperty, owl:ObjectProperty;
  rdfs:label "insertedContentRelation";
  rdfs:domain ldp:IndirectContainerRule;
  rdfs:range  rdf:Property .

### 
ldp:HTTPActionRule a rdfs:Class;
   rdfs:comment """
      a rule on what consequences will occur on POSTing to a container.
   """.

ldp:bindingRule a rdf:Property, owl:ObjectProperty;
   rdfs:label "binding rule";
   rdfs:domain ldp:Container;
   rdfs:range ldp:HTTPActionRule .

ldp:IndirectContainerRule rdfs:subClassOf ldp:HTTPActionRule, 
                   [ a owl:Restriction;
                     owl:onProperty ldp:hasMemberRelation;
                     owl:cardinality 1;
                   ],
                   [ a owl:Restriction;
                     owl:onProperty ldp:insertedContentRelation;
                     owl:cardinality 1;
                   ],
                   [ a owl:Restriction;
                     owl:onProperty ldp:membershipResource;
                     owl:cardinality 1;
                   ].

ldp:DirectContainerRule owl:equivalentClass [ a owl:Restriction;
                     owl:onProperty ldp:insertedContentRelation;
                     owl:hasValue ldp:MemberSubject
                    ]. 

ldp:ContainerRule owl:equivalentClass [ owl:intersectionOf ( 
                [ a owl:Restriction;
                  owl:onProperty [ 
                    owl:subPropertyOf 
                      [ owl:propertyChainAxiom ( ldp:memberResource ldp:bindingRule ) ];
                    ];
                 owl:hasSelf "true"^^xsd:boolean ]
                [ a owl:Restriction;
                 owl:onProperty ldp:hasMemberRelation;
                 owl:hasValue ldp:contains ] 
                [ a owl:Restriction;
                 owl:onProperty ldp:insertedContentRelation;
                 owl:hasValue ldp:MemberSubject
                ])];
   rdfs:label "ContainerRule";
   rdfs:comment """
     the rule that on POSTing creates an ldp:contains relation, etc... 
   """.


ldp:Container 
   rdfs:subClassOf [ a owl:Restriction;
         owl:onProperty ldp:bindingRule;
         owl:someValuesFrom ldp:ContainerRule ].

ldp:IndirectContainer 
    rdfs:subClassOf  [ a owl:Restriction; 
              owl:onProperty ldp:bindingRule;
              owl:maxQualifiedCardinality 2;
              owl:onClass ldp:IndirectContainerRule ]. 

ldp:DirectContainer 
    rdfs:subClassOf [  a owl:Restriction; 
              owl:onProperty ldp:bindingRule;
              owl:maxQualifiedCardinality 2;
              owl:onClass ldp:DirectContainerRule 
             ]. 

ldp:BasicContainer 
   owl:equivalentClass [ a owl:Restriction;
         owl:onProperty ldp:bindingRule;
         owl:qualifiedCardinality 1;
         owl:onClass ldp:ContainerRule ] .

