@prefix rdf: <http://www.w3.org/1999/02/22-rdf-syntax-ns#> .
@prefix owl: <http://www.w3.org/2002/07/owl#> .
@prefix rdfs: <http://www.w3.org/2000/01/rdf-schema#> .
@prefix skos: <http://www.w3.org/2004/02/skos/core#> .
@prefix ldp: <http://www.w3.org/ns/ldp#> .
@prefix xsd: <http://www.w3.org/2001/XMLSchema#>.


ldp:Resource a rdfs:Class;
  rdfs:label "ldp Resource";
  rdfs:comment """
     A HTTP resource whose state is represented in any way that conforms to the simple 
     lifecycle patterns and conventions in section 5. Linked Data Platform Resources.
  """ .

ldp:Source a rdfs:Class;
  rdfs:label "ldp Resource";
  rdfs:subClassOf ldp:Resource;
  rdfs:comment """
    an ldp:Resource that is also an rdf source: ie that is an RDF graph.
  """ .

ldp:Container a rdfs:Class, owl:Class;
  rdfs:label "ldp Container";
  rdfs:subClassOf ldp:Source;
  rdfs:comment """
    An LDPR representing a collection of member resources and/or contained documents 
    (RDF Document [rdf11-concepts]  or information resources [WEBARCH]) that responds 
    to client requests for creation, modification, and/or enumeration 
    of its members and documents, and that conforms to the simple lifecycle patterns 
    and conventions in section6. Linked Data Platform Containers.
  """;
  skos:editorialNote """
    As the outermost class of the container hierarchy it may be that the ldp:Container could 
be made to be the same as the ldp:IndirectContainer. But leaving space could allow for further
extensions.    
  """ .

ldp:IndirectContainer a rdfs:Class, owl:Class;
   rdfs:comment """
   A LDPC that has the flexibility of choosing what form its membership triples take, 
   and allows members to be any resources [WEBARCH], defined in the posted document.
   """ .

ldp:DirectContainer a rdfs:Class, owl:Class;
   rdfs:comment """
   A LDPC that has the flexibility of choosing what form its membership triples take, 
   and allows members to be any resources [WEBARCH], not only documents.
   """ .

ldp:BasicContainer a rdfs:Class, owl:Class;
  rdfs:label "BasicContainer";
  rdfs:comment """
  A LDPC that uses a single pre-defined predicate to link to both its contained and 
  member documents (information resources). Posting to an ldp:BasicContainer has
  no extra consequences other than creating an ldp:contains relation from the container to
  the newly created resource.
  """ .
 
ldp:contains a rdf:Property, owl:ObjectProperty;
  rdfs:label "contains";
  rdfs:domain ldp:Container;
  rdfs:range ldp:Resource;
  rdfs:comment """
    the ldp:contains relation relates an ldp:Container to a ldp:Resource ( ie a document of some form )
  """ .

ldp:membershipResource a rdf:Property, owl:FunctionalProperty;
  rdfs:label "membershipResource";
  owl:propertyChainAxiom ( ldp:bindingRule ldp:subject ) ;
  rdfs:domain ldp:IndirectBindingRule;
  rdfs:range  rdfs:Resource .

ldp:hasMemberRelation a rdf:Property, owl:FunctionalProperty, owl:ObjectProperty;
  rdfs:label "hasMemberRelation";
  owl:propertyChainAxiom ( ldp:bindingRule ldp:relation ) ;
  rdfs:domain ldp:IndirectBindingRule;
  rdfs:range  rdf:Property .
  

ldp:isMemberOfRelation a rdf:Property, owl:FunctionalProperty, owl:ObjectProperty; 
   rdfs:label "isMemberOfRelation";
   owl:propertyChainAxiom ( ldp:hasMemberRelation owl:inverseOf ) ;
   skos:editorialNote """
      the ldp:isMemberOfRelation is the equivalent to the hasMemberRelation followed by the owl:inverseOf property 
   """;
   rdfs:range rdf:Property .

ldp:insertedContentRelation a owl:FunctionalProperty, owl:ObjectProperty;
  rdfs:label "insertedContentRelation";
  owl:propertyChainAxiom ( ldp:bindingRule ldp:contentRelation ) ;
  rdfs:range  rdf:Property .

### 
#
# New rules based framework 
#
### 

ldp:HTTPActionRule a rdfs:Class;
   rdfs:comment """
      a rule on what consequences will occur on POSTing to a container.
   """.

ldp:bindingRule a rdf:Property, owl:ObjectProperty;
   rdfs:label "binding rule";
   rdfs:domain ldp:Container;
   rdfs:range ldp:HTTPActionRule .

ldp:subject a rdf:Property, owl:FunctionalProperty;
  rdfs:label "rule subject";
  rdfs:domain ldp:IndirectBindingRule;
  rdfs:range  rdfs:Resource .

ldp:relation a rdf:Property, owl:FunctionalProperty, owl:ObjectProperty;
  rdfs:label "rule relation";
  rdfs:domain ldp:IndirectBindingRule;
  rdfs:range  rdf:Property .

ldp:contentRelation a owl:FunctionalProperty, owl:ObjectProperty;
  rdfs:label "content relation";
  rdfs:domain ldp:IndirectBindingRule;
  rdfs:range  rdf:Property .

ldp:IndirectBindingRule rdfs:subClassOf ldp:HTTPActionRule, 
                   [ a owl:Restriction;
                     owl:onProperty ldp:subject;
                     owl:cardinality 1;
                   ],
                   [ a owl:Restriction;
                     owl:onProperty ldp:relation;
                     owl:cardinality 1;
                   ],
                   [ a owl:Restriction;
                     owl:onProperty ldp:contentRelation;
                     owl:cardinality 1;
                   ].

ldp:DirectBindingRule owl:equivalentClass [ a owl:Restriction;
                     owl:onProperty ldp:contentRelation;
                     owl:hasValue ldp:MemberSubject
                    ]. 

ldp:subjectToBindingRule a rdf:Property;
#   owl:propertyChainAxiom ( ldp:subject ldp:bindingRule );
   rdfs:comment """
     artificial relation needed for ldp:ContainerRule owl:Restriction.
     This enables on to specify a relation from a subject to a bindingrule, so that
    one can set an owl:hasSelf restriction
   """.

ldp:ContainerRule owl:equivalentClass [ owl:intersectionOf ( 
                [ a owl:Restriction;
                  rdfs:comment """
                    This restrictions is attempting to state that if one follows the
                 property subject then bindingRule one will arrive at the same object
                 again at least once. That should be equivalent to saying that for this class
                 of objects the :subject relation is the same as the subject of the :bindingRule
                 relation.
                 """;
# problem with pellet reasoning on properties defined via property chains
                  owl:onProperty owl:reflexiveSubjectToBindingRule;
#                 Pellet does not like the following:
#                 owl:onProperty [ rdfs:subPropertyOf ldp:subjectToBindingRule;
#                                  a owl:ReflexiveProperty ];
                  owl:minCardinality 1 ]
                [ a owl:Restriction;
                  owl:onProperty ldp:relation;
                  owl:hasValue ldp:contains ] 
                [ a owl:Restriction;
                  owl:onProperty ldp:contentRelation;
                  owl:hasValue ldp:MemberSubject
                ])];
   rdfs:label "ContainerRule";
   rdfs:comment """
     the rule that on POSTing creates an ldp:contains relation, etc... 
   """.


ldp:Container 
   rdfs:comment "a Container has 1 ContainerRule ( and may have others )";
   owl:equivalentClass [ a owl:Restriction;
         owl:onProperty ldp:bindingRule;
         owl:qualifiedCardinality 1;
         owl:onClass ldp:ContainerRule ].

ldp:IndirectContainer 
    rdfs:comment """
     an IndirectContainer has at most 2 binding rules of which 1 IndirectBindingRule 
   ( and since it has a bindingRule it is a Container too ) 
    """;
    owl:equivalentClass [ owl:intersectionOf (
            [ a owl:Restriction;
              owl:onProperty ldp:bindingRule;
              owl:maxCardinality 2 ]
            [ a owl:Restriction; 
              owl:onProperty ldp:bindingRule;
              owl:qualifiedCardinality 1;
              owl:onClass ldp:IndirectBindingRule ]
            )
      ]. 

ldp:DirectContainer 
    rdfs:comment """
     an DirectContainer has at most 2 biding rules of which 1 DirectBindingRule 
   ( and since it has a bindingRule it is a Container too )
    """;
     owl:equivalentClass [ owl:intersectionOf (
            [ a owl:Restriction;
              owl:onProperty ldp:bindingRule;
              owl:maxCardinality 2 ]
            [  a owl:Restriction; 
              owl:onProperty ldp:bindingRule;
              owl:qualifiedCardinality 1;
              owl:onClass ldp:DirectBindingRule ]
           )
      ]. 

ldp:BasicContainer 
   rdfs:comment "a BasicContainer only has one bindingRule - and so the ContainerRule";
   owl:equivalentClass [ a owl:Restriction;
         owl:onProperty ldp:bindingRule;
         owl:cardinality 1 ] .

## example
@base <http://example.org/> .
@prefix ex: <http://example/> .
@prefix sioc: <http://rdfs.org/sioc/ns#> .
 
</2014/> a ldp:DirectContainer;
      ldp:bindingRule [ a ldp:DirectBindingRule;
               ldp:relation sioc:container_of;
               ldp:subject </2014/>;
            ];
      ldp:contains </2014/e1>;
      sioc:container_of </2014/e1> .
 
# sioc:has_container owl:inverseOf ldp:contains .
# 

@prefix dcterms: <http://purl.org/dc/terms/>.
@prefix o: <http://example.org/ontology/>.

</netWorth/> a ldp:DirectContainer;
   dcterms:title "The assets of JohnZSmith";
   ldp:bindingRule [ a ldp:DirectBindingRule;
        ldp:subject </netWorth/nw1/>;
        ldp:relation o:asset;
      ];
   ldp:contains </netWorth/a1>, </netWorth/a2> .
